wip

theories/examples/counterexample.v
@@ -1,34 +1,35 @@
-From clutch Require Export clutch lib.flip.
+(** If we assume that we can freely pick presampling tapes to read from when *)
+(*     resolving probabilistic choices, we can show refinements/equivalences that *)
+(*     do not hold. *)
+From clutch Require Export clutch lib.flip lib.conversion.
 Set Default Proof Using "Type*".
 
-(** If we assume that we can freely pick presampling tapes to read from when
-    resolving probabilistic choices, we can show refinements/equivalences that
-    do not hold. *)
+(** An (unsound) rule that allows us to pick an arbitrary presampling tape when
+    resolving the [flip] on the left. *)
+Definition refines_tape_unsound `{!clutchRGS Σ} :=
+  ∀ K E A α b bs e',
+    α ↪B (b :: bs) ∗
+    (α ↪B bs -∗ REL fill K (of_val #b) << e' @ E : A)
+    ⊢ REL fill K flip << e' @ E : A.
+
+
 Section counterexample.
   Context `{!clutchRGS Σ}.
 
-  (** An (unsound) rule that allows us to pick an arbitrary presampling tape
-      when resolving the [flip] on the left. *)
-  Definition refines_tape_unsound :=
-    ∀ K E (A : lrel Σ) α b bs e',
-    α ↪B (b :: bs) ∗
-    (α ↪B bs -∗  REL fill K (of_val #b) << e' @ E : A)
-    ⊢ REL fill K flip << e' @ E : A.
-
-  (** [flip_ors] return [true] with probability 3/4, false with 1/4 *)
+  (** [flip_ors] returns [true] with probability 3/4, false with 1/4 *)
   Definition flip_ors : expr :=
     let: "x" := flip in
     let: "y" := flip in
     "x" || "y".
 
-  (** If we assume [refines_tape_unsound], we can show that [flip] refines
-      [flip_ors] which obviously cannot true. *)
+  (** If we assume [refines_tape_unsound], we can show that [flip] refines 
+      [flip_ors] which obviously cannot be true. *)
   Lemma counterexample α1 α2 :
     refines_tape_unsound →
     α1 ↪B [] ∗ α2 ↪B []
     ⊢ REL flip << flip_ors  : lrel_bool.
   Proof.
-    iIntros (refines_tape_unsound) "[Hα1 Hα2]". rewrite /flip_ors.
+    iIntros (Hrule) "[Hα1 Hα2]". rewrite /flip_ors.
     rel_apply (refines_couple_tape_flip _ _ α1); [done|iFrame].
     iIntros (b1) "Hα1 /=".
     rel_pures_r.
@@ -36,10 +37,200 @@ Section counterexample.
     iIntros (b2) "Hα2 /=".
     rel_pures_r.
     destruct b1; rel_pures_r.
-    - rel_apply (refines_tape_unsound _ _ _ α1).
+    - rel_apply (Hrule _ _ _ α1).
       iFrame. iIntros "Hα1". rel_values.
-    - rel_apply (refines_tape_unsound _ _ _ α2).
+    - rel_apply (Hrule _ _ _ α2).
       iFrame. iIntros "Hα2". rel_values.
   Qed.
 
 End counterexample.
+
+Definition flip' : expr :=
+  let: "α1" := allocB in
+  let: "α2" := allocB in
+  flip.
+
+Lemma counterexample_ctx :
+  (∀ `{clutchRGS Σ}, refines_tape_unsound) →
+  ∅ ⊨ flip' ≤ctx≤ flip_ors : TBool.
+Proof.
+  intros Hrule.
+  eapply (refines_sound clutchRΣ).
+  iIntros (??). rewrite /flip'.
+  rel_allocBtape_l α1 as "Hα1".
+  rel_allocBtape_l α2 as "Hα2".
+  rel_pures_l. rewrite -/flip.
+  by iApply (counterexample with "[$]").
+Qed.
+
+(* just rewriting with [dret_id_left] unfolds [exec_val] even though its
+   opaque.... *)
+Local Ltac rem_dret_left :=
+  match goal with
+  | |- context[dbind (exec_val ?n) (dret ?ρ)] =>
+      replace (dbind _ (dret _)) with (exec_val n ρ)
+  end; [|rewrite dret_id_left //].
+
+Local Opaque exec_val.
+
+Lemma exec_val_flip' σ :
+  exec_val 11 (flip', σ) = fair_conv_comb (dret #true) (dret #false).
+Proof.
+  rewrite /flip'.
+
+  rewrite exec_val_Sn_not_val //=.
+  reshape_prim_step allocB.
+  rewrite dmap_dret /=.
+  rem_dret_left.
+
+  rewrite exec_val_Sn_not_val //=.
+  reshape_prim_step (λ: _, _)%E.
+  rewrite dmap_dret /=.
+  rem_dret_left.
+
+  rewrite exec_val_Sn_not_val //=.
+  rewrite head_prim_step_eq /=; [|eauto with head_step].
+  rem_dret_left.
+
+  rewrite exec_val_Sn_not_val //=.
+  reshape_prim_step allocB.
+  rewrite dmap_dret /=.
+  rem_dret_left.
+  set (σ' := {| heap := _; tapes := _ |}).
+
+  rewrite exec_val_Sn_not_val //=.
+  reshape_prim_step (λ: _, _)%E.
+  rewrite dmap_dret /=.
+  rem_dret_left.
+
+  rewrite exec_val_Sn_not_val //=.
+  rewrite head_prim_step_eq /=; [|eauto with head_step].
+  rem_dret_left.
+
+  rewrite -/flip.
+  apply exec_val_flip.
+Qed.
+
+Lemma exec_val_flip'_obs σ (b : bool) :
+  exec_val 11 (flip', σ) #b = 0.5%R.
+Proof.
+  rewrite exec_val_flip'.
+  rewrite fair_conv_comb_pmf.
+  destruct b.
+  - rewrite dret_1_1 // dret_0 //. lra.
+  - rewrite dret_0 // dret_1_1 //. lra.
+Qed.
+
+Tactic Notation "reshape_prim_step'" open_constr(efoc) :=
+  lazymatch goal with
+  | |- context[prim_step ?e _] =>
+      reshape_expr e
+        ltac:(fun K e' =>
+                unify e' efoc;
+                rewrite (fill_prim_step_dbind K e') //)
+  end.
+
+Local Lemma bias_leq :
+ (0 <= 0.75 <= 1)%R.
+Proof. lra. Qed.
+
+Lemma exec_is_val e σ n :
+  is_Some (to_val e) →
+  exec n (e, σ) = dret (e, σ).
+Proof.
+  induction n. 
+  { rewrite exec_O //. }
+  intros Hv.
+  rewrite exec_Sn.
+  rewrite prim_step_or_val_is_val //.
+  rewrite dret_id_left.
+  rewrite -IHn //.
+Qed. 
+  
+Lemma exec_val_exec n m (ρ : cfg) :
+  exec_val (n + m) ρ = dbind (λ ρ', exec_val m ρ') (exec n ρ). 
+Proof.
+  revert ρ. 
+  induction n.
+  { intros. rewrite exec_O /= dret_id_left //. }
+  intros [e σ]=>/=.
+  destruct (to_val e) eqn:Heq.
+  - erewrite exec_val_is_val; [|done]. 
+    rewrite exec_Sn.
+    rewrite prim_step_or_val_is_val //.
+    replace (dbind (exec n) (dret (e, σ)))
+      with (exec n (e, σ)); [|rewrite dret_id_left //].
+    rewrite exec_is_val //.
+    rewrite dret_id_left.
+    by erewrite exec_val_is_val.
+  - rewrite exec_val_Sn_not_val //=.
+    rewrite exec_Sn.
+    rewrite prim_step_or_val_no_val //=.
+    rewrite -dbind_assoc. 
+    apply dbind_eq; [|auto].
+    intros ρ.
+    intros Hs. rewrite IHn //.
+Qed. 
+
+Lemma exec_plus_bind K `{!LanguageCtx K} n m (e : expr) σ :
+  exec (n + m) (K e, σ) = dbind (λ '(e', σ'), exec m (K e', σ')) (exec n (e, σ)).
+Proof.
+  revert e σ.
+      
+Admitted. 
+
+Lemma exec_val_flip_ors σ :
+  exec_val 14 (flip_ors, σ) = biased_conv_comb 0.75%R bias_leq (dret #true) (dret #false).
+Proof.
+  rewrite /flip_ors.
+  rewrite (exec_val_exec 12 2) /=.
+  
+  rewrite exec_Sn.
+  rewrite prim_step_or_val_no_val //=.
+  reshape_prim_step' flip.
+  
+
+Admitted.
+
+Lemma exec_val_flip_ors_obs σ  :
+  exec_val 14 (flip_ors, σ) #false = 0.25%R.
+Proof.
+  rewrite exec_val_flip_ors.
+  rewrite biased_conv_comb_pmf.
+  rewrite dret_0 // dret_1_1 //. lra.
+Qed.
+
+Lemma counterexample_False :
+  (∀ `{clutchRGS Σ}, refines_tape_unsound) → False.
+Proof.
+  intros Hctx%counterexample_ctx.
+  set (σ0 := {| heap := ∅; tapes := ∅ |}).
+  specialize (Hctx [] σ0 false (TPCTX_nil ∅ _)).
+  simpl in *.
+  assert (lim_exec_val (flip', σ0) #false = 0.5)%R as Hflip.
+  { rewrite (lim_exec_positive_ast 11); [apply exec_val_flip'_obs|].
+    rewrite exec_val_flip'.
+    (* TODO: extract this as a general lemma about [fair_conv_comb]*)
+    rewrite /fair_conv_comb.
+    rewrite /pmf /= /dbind_pmf.
+    rewrite distr_double_swap.
+    setoid_rewrite SeriesC_scal_l.
+    setoid_rewrite (SeriesC_ext _ (λ b, fair_coin b)) ; last first.
+    { intros []; rewrite dret_mass; lra. }
+    rewrite SeriesC_finite_mass/=. lra. }
+  assert (lim_exec_val (flip_ors, σ0) #false = 0.25)%R as Hflip_ors.
+  { rewrite (lim_exec_positive_ast 14); [apply exec_val_flip_ors_obs|].
+    rewrite exec_val_flip_ors.
+    rewrite /biased_conv_comb /pmf /= /dbind_pmf.
+    rewrite distr_double_swap.
+    setoid_rewrite SeriesC_scal_l.
+    setoid_rewrite (SeriesC_ext _ (λ b, biased_coin 0.75 bias_leq b)) ; last first.
+    { intros []; rewrite dret_mass; lra. }
+    rewrite (SeriesC_ext _ (λ b, (if bool_decide (b = true) then 0.75 else 0) +
+                                  if bool_decide (b = false) then 0.25 else 0))%R.
+    2: { intros []; rewrite /= {1}/pmf /=;  lra. }
+    erewrite SeriesC_plus; [|eapply ex_seriesC_singleton.. ].
+    rewrite 2!SeriesC_singleton /=. lra. }
+  rewrite Hflip Hflip_ors in Hctx.
+  lra.
+Qed.
