theories/prob_lang/primitive_laws.v
@@ -122,7 +122,6 @@ Proof.
   iApply wp_lift_atomic_head_step; [done|].
   iIntros (σ1) "Hσ !#".
   iSplit; [eauto with head_step|].
-  Unshelve. 2 : { apply 0%fin . }
   iIntros "!>" (e2 σ2 Hs).
   inv_head_step.
   iFrame.
@@ -169,8 +168,7 @@ Proof.
   iApply wp_lift_atomic_head_step; [done|].
   iIntros (σ1) "(Hh & Ht) !#".
   iDestruct (ghost_map_lookup with "Ht Hl") as %?.
-  iSplit; [by eauto with head_step|].
-  Unshelve. 2 : { apply 0%fin. }
+  iSplit; [eauto with head_step|].
   iIntros "!>" (e2 σ2 Hs).
   inv_head_step.
   iFrame.
@@ -186,8 +184,7 @@ Proof.
   iApply wp_lift_atomic_head_step; [done|].
   iIntros (σ1) "(Hh & Ht) !#".
   iDestruct (ghost_map_lookup with "Ht Hl") as %?.
-  iSplit; [by eauto with head_step|].
-  Unshelve. 2 : { apply 0%fin. }
+  iSplit; [eauto with head_step|].
   iIntros "!>" (e2 σ2 Hs).
   inv_head_step.
   iFrame.
@@ -196,5 +193,3 @@ Proof.
 Qed.  
 
 End lifting.
-
-Global Hint Extern 0 (TCEq _ (Z.to_nat _ )) => rewrite Nat2Z.id : typeclass_instances. 
